src/named/Substable.v
@@ -1,0 +1,121 @@
+Set Implicit Arguments.
+Set Bullet Behavior "Strict Subproofs".
+
+Require Import List.
+Import ListNotations.
+Open Scope list.
+From Utils Require Import Utils.
+
+Section WithVar.
+  Context (V : Type).
+
+  Notation named_list := (@named_list V).
+  Notation named_map := (@named_map V).
+
+
+  (* Operations for types that can be substituted into themselves *)
+  Class Substable0 (A : Type) : Type :=
+    {
+      inj_var : V -> A;
+      apply_subst0 : named_list A -> A -> A;
+      well_scoped0 : list V -> A -> Prop;
+    }.
+
+  Section WithSubstable0.
+    Context {A} {Substable0 : Substable0 A}.
+
+    Notation subst := (named_list A).
+
+    Definition id_args {B} (c : named_list B) :=
+      map inj_var (map fst c).
+
+    (*Defined as a notation so that the definition 
+      does not get in the way of automation *)
+    Notation id_subst c := (with_names_from c (id_args c)).
+    
+    Definition subst_cmp (s1 s2 : named_list A) := named_map (apply_subst0 s1) s2.
+
+    Fixpoint ws_subst args (s : subst) : Prop :=
+      match s with
+      | [] => True
+      | (n,e)::s' => fresh n s' /\ well_scoped0 args e /\ ws_subst args s'
+      end.
+    Arguments ws_subst args !s/.
+
+    Class Substable0_ok : Type :=
+      {
+        subst_assoc0 : forall s1 s2 a,
+          well_scoped0 (map fst s2) a ->
+          apply_subst0 s1 (apply_subst0 s2 a) = apply_subst0 (subst_cmp s1 s2) a;
+        subst_id0 : forall {A} (c : named_list A) a,
+          (* Not necessary because of our choice of default
+        well_scoped (map fst c) a ->*)
+          apply_subst0 (id_subst c) a = a;
+        strengthen_subst0
+        : forall s a n e,
+          well_scoped0 (map fst s) a ->
+          fresh n s ->
+          apply_subst0 ((n,e)::s) a = apply_subst0 s a;
+        well_scoped_subst0 args s a
+        : ws_subst args s ->
+          well_scoped0 (map fst s) a ->
+          well_scoped0 args (apply_subst0 s a)
+      }.
+
+    Class Substable (B : Type) : Type :=
+      {
+        apply_subst : subst -> B -> B;
+        well_scoped : list V -> B -> Prop;
+        subst_assoc : forall s1 s2 a,
+          well_scoped (map fst s2) a ->
+          apply_subst s1 (apply_subst s2 a) = apply_subst (subst_cmp s1 s2) a;
+        subst_id : forall {B} (c : named_list B) a,
+          (* Not necessary because of our choice of default
+        well_scoped (map fst c) a ->*)
+          apply_subst (id_subst c) a = a;
+        strengthen_subst
+        : forall s a n e,
+          well_scoped (map fst s) a ->
+          fresh n s ->
+          apply_subst ((n,e)::s) a= apply_subst s a;
+        well_scoped_subst args s a
+        : ws_subst args s ->
+          well_scoped (map fst s) a ->
+          well_scoped args (apply_subst s a)
+      }.
+
+  End WithSubstable0.
+
+  
+  #[export] Instance substable0_is_substable {A} `{Substable0 A} `{Substable0_ok A}
+    : Substable A :=
+    {
+      apply_subst := apply_subst0;
+      well_scoped := well_scoped0;
+      subst_assoc :=  subst_assoc0;
+      subst_id := @subst_id0 _ _ _;
+      strengthen_subst := strengthen_subst0;
+      well_scoped_subst := well_scoped_subst0;
+    }.
+
+End WithVar.
+
+Arguments id_args : simpl never.
+
+(*Defined as a notation so that the definition 
+does not get in the way of automation *)
+Notation id_subst c := (with_names_from c (id_args c)).
+
+Arguments Substable0_ok [V]%type_scope _%type_scope {_}.
+Arguments Substable {V}%type_scope _%type_scope {_} _%type_scope.
+
+Arguments well_scoped [V]%type_scope {A}%type_scope {_} {B}%type_scope {_} _%list_scope !_.
+Arguments apply_subst [V]%type_scope {A}%type_scope {_} {B}%type_scope {_} _%list_scope !_.
+
+(*TODO: add'l arguments, fix these hints*)
+#[global] Hint Rewrite @subst_assoc : term.
+#[global] Hint Rewrite @subst_id : term.
+#[global] Hint Rewrite @strengthen_subst : term.
+#[global] Hint Resolve well_scoped_subst : term.
+
+Notation "e [/ s /]" := (apply_subst s e) (at level 7, left associativity).
